src/ILTP/main.ml
@@ -1,16 +1,18 @@
 let file = ref ""
 let dir = ref ""
 let ext = ref ""
+let header = ref ""
+let map_char c = match c with '+' -> '_' | '.' -> '_' | c -> c
+let normalise_str str = String.map map_char str
 
-let process_file str =
+let process_file hd str =
   try
     let ifile = open_in str in
-    let vfile = open_out (Filename.chop_extension str ^ ".v") in
+    let vfile = open_out (normalise_str (Filename.chop_extension str) ^ ".v") in
     let lexbuf = Lexing.from_channel ifile in
     let b, l = Parser.file Lexer.token lexbuf in
-    List.iter (fun f -> Printf.fprintf vfile "%a\n" Formula.output_formula f) l;
-    if b then output_string vfile "Proof. tauto. Qed.\n"
-    else output_string vfile "Proof. Fail intuition fail. Abort.\n";
+    Printf.fprintf vfile "%s\n" hd;
+    Formula.output_file vfile (b, l);
     close_out_noerr vfile;
     close_in_noerr ifile
   with
@@ -18,20 +20,21 @@ let process_file str =
   | Parsing.Parse_error ->
     raise (failwith (Printf.sprintf "%s : Parse_error" str))
 
-let rec process_dir ext dname =
+let rec process_dir hd ext dname =
   Array.iter
     (fun s ->
       let fn = Filename.concat dname s in
-      if Sys.is_directory fn then process_dir ext fn
-      else if Filename.check_suffix fn ext then process_file fn)
+      if Sys.is_directory fn then process_dir hd ext fn
+      else if Filename.check_suffix fn ext then process_file hd fn)
     (Sys.readdir dname)
 
 let args =
   [ ("-ifile", Arg.Set_string file, "File to parse")
   ; ("-idir", Arg.Set_string dir, "Directory to analyse")
-  ; ("-ext", Arg.Set_string ext, "File extension") ]
+  ; ("-ext", Arg.Set_string ext, "File extension")
+  ; ("-header", Arg.Set_string header, "Header string to insert") ]
 
 let _ =
   Arg.parse args (fun s -> ()) "";
-  if !file <> "" then process_file !file
-  else if !dir <> "" && !ext <> "" then process_dir !ext !dir
+  if !file <> "" then process_file !header !file
+  else if !dir <> "" && !ext <> "" then process_dir !header !ext !dir
