Makefile
@@ -1,6 +1,10 @@
 all : CoqMakefile
 	make -f CoqMakefile
 
+prover :theories/Formula.v
+	find . -name prover.cmi -exec rm {} \;
+	find . -name prover.mli -exec rm {} \;
+
 install :
 	make -f CoqMakefile install
 
